coq/FwOF/FwOFSignatures.v
@@ -1,0 +1,757 @@
+Set Implicit Arguments.
+
+Require Import Coq.Lists.List.
+Require Import Coq.Structures.Equalities.
+Require Import Coq.Classes.Equivalence.
+Require Import Coq.Classes.EquivDec.
+Require Import Common.Types.
+Require Import Bag.Bag.
+Require Import Common.AllDiff.
+Require Import Common.Bisimulation.
+
+Local Open Scope list_scope.
+Local Open Scope equiv_scope.
+Local Open Scope bag_scope.
+
+Module Type NETWORK_ATOMS.
+
+  Parameter packet : Type.
+  Parameter switchId : Type.
+  Parameter portId : Type.
+  Parameter flowTable : Type.
+  Parameter flowMod : Type.
+
+  Inductive fromController : Type :=
+  | PacketOut : portId -> packet -> fromController
+  | BarrierRequest : nat -> fromController
+  | FlowMod : flowMod -> fromController.
+
+  Inductive fromSwitch : Type :=
+  | PacketIn : portId -> packet -> fromSwitch
+  | BarrierReply : nat -> fromSwitch.
+
+  (** Produces a list of packets to forward out of ports, and a list of packets
+      to send to the controller. *)
+  Parameter process_packet : flowTable -> portId -> packet -> 
+    list (portId * packet) * list packet.
+
+  Parameter modify_flow_table : flowMod -> flowTable -> flowTable.
+
+  Parameter packet_eq_dec : Eqdec packet.
+  Parameter switchId_eq_dec : Eqdec switchId.
+  Parameter portId_eq_dec : Eqdec portId.
+  Parameter flowTable_eq_dec : Eqdec flowTable.
+  Parameter flowMod_eq_dec : Eqdec flowMod.
+  Declare Instance Eq_switchId : Eq switchId.
+  Declare Instance Eq_portId : Eq portId.
+  Declare Instance Eq_packet : Eq packet.
+
+  Instance EqDec_switchId : EqDec switchId eq := eqdec.
+  Instance EqDec_portId : EqDec portId eq := eqdec.
+  Instance EqDec_packet : EqDec packet eq := eqdec. 
+
+End NETWORK_ATOMS.
+
+Module Type NETWORK_AND_POLICY <: NETWORK_ATOMS.
+
+  Include Type NETWORK_ATOMS.
+
+  Parameter topo : switchId * portId -> option (switchId * portId).
+  Parameter abst_func : switchId -> portId -> packet -> list (portId * packet).
+
+End NETWORK_AND_POLICY.
+
+(** Elements of a Featherweight OpenFlow model. *)
+Module Type ATOMS <: NETWORK_AND_POLICY.
+
+  Include NETWORK_AND_POLICY.
+
+  Parameter controller : Type.
+
+  Parameter controller_recv : controller -> switchId -> fromSwitch -> 
+    controller -> Prop.
+
+  Parameter controller_step : controller -> controller -> Prop.
+
+  Parameter controller_send : controller ->  controller -> switchId -> 
+    fromController -> Prop.
+
+End ATOMS.
+
+Module Type MACHINE.
+
+  Declare Module Atoms : ATOMS.
+  Import Atoms.
+
+  Existing Instances  Eq_switchId Eq_portId Eq_packet EqDec_switchId
+     EqDec_portId EqDec_packet.
+
+  Parameter fromController_eq_dec : Eqdec fromController.
+  Parameter fromSwitch_eq_dec : Eqdec fromSwitch.
+  Declare Instance FromController_Eq : Eq fromController.
+  Declare Instance FromSwitch_Eq : Eq fromSwitch.
+  Declare Instance FlowTable_Eq : Eq flowTable.
+  Instance fromController_eqdec : EqDec fromController eq := eqdec.
+  Instance fromSwitch_eqdec : EqDec fromSwitch eq := eqdec.
+
+  (* Field names have two purposes. Coq creates selectors with these names,
+     and also uses them to generate variable names in proofs. We spend
+     more time in FwOF proofs, so we pick short names here. *)
+  Record switch := Switch {
+    swId : switchId;
+    pts : list portId;
+    tbl : flowTable;
+    inp : bag (portId * packet);
+    outp :  bag (portId * packet);
+    ctrlm : bag fromController;
+    switchm : bag fromSwitch
+  }.
+  
+  Record dataLink := DataLink {
+    src : switchId * portId;
+    pks : list packet;
+    dst : switchId * portId
+  }.
+  
+  Record openFlowLink := OpenFlowLink {
+    of_to : switchId;
+    of_switchm : list fromSwitch;
+    of_ctrlm : list fromController
+  }.
+
+  Definition observation := (switchId * portId * packet) %type.
+
+  (* NOTE(arjun): Ask me in person why exactly I picked these levels. *)
+  Reserved Notation "SwitchStep[ sw ; obs ; sw0 ]"
+    (at level 70, no associativity).
+  Reserved Notation "ControllerOpenFlow[ c ; l ; obs ; c0 ; l0 ]"
+    (at level 70, no associativity).
+  Reserved Notation "TopoStep[ sw ; link ; obs ; sw0 ; link0 ]"
+    (at level 70, no associativity).
+  Reserved Notation "SwitchOpenFlow[ s ; l ; obs ; s0 ; l0 ]"
+    (at level 70, no associativity).
+
+  Inductive NotBarrierRequest : fromController -> Prop :=
+  | PacketOut_NotBarrierRequest : forall pt pk,
+      NotBarrierRequest (PacketOut pt pk)
+  | FlowMod_NotBarrierRequest : forall fm,
+      NotBarrierRequest (FlowMod fm).
+
+  (** Devices of the same type do not interact in a single
+      step. Therefore, we never have to permute the lists below. If we
+      instead had just one list of all devices, we would have to worry
+      about permuting the list or define symmetric step-rules. *)
+  Record state := State {
+    switches : bag switch;
+    links : list dataLink;
+    ofLinks : list openFlowLink;
+    ctrl : controller
+  }.
+
+  (** Switches contain bags and bags do not have unique representations. In
+      proofs, it is common to replace a bag with an equivalent (but unequal)
+      bag. When we do, we need to replace the switch with an equivalent switch
+      too. *)
+
+  Inductive switch_equiv : switch -> switch -> Prop :=
+  | SwitchEquiv : forall swId pts tbl inp inp' outp outp' ctrlm ctrlm'
+                         switchm switchm',
+    inp === inp' ->
+    outp === outp' ->
+    ctrlm  === ctrlm' ->
+    switchm === switchm' ->
+    switch_equiv (Switch swId pts tbl inp outp ctrlm switchm)
+                 (Switch swId pts tbl inp' outp' ctrlm' switchm').
+
+  Parameter switch_equiv_is_Equivalence : Equivalence switch_equiv.
+  
+  Instance switch_Equivalence : Equivalence switch_equiv := 
+    switch_equiv_is_Equivalence.
+  
+  Parameter switch_eqdec : EqDec switch switch_equiv.
+  
+  Inductive stateEquiv : state -> state -> Prop :=
+  | StateEquiv : forall sws1 sws2 links ofLinks ctrl,
+    sws1 === sws2 ->
+    stateEquiv
+      (State sws1 links ofLinks ctrl) 
+      (State sws2 links ofLinks ctrl).
+  
+  Parameter stateEquiv_is_Equivalence : Equivalence stateEquiv.
+
+  Instance stateEquiv_Equivalence : Equivalence stateEquiv :=
+    stateEquiv_is_Equivalence.
+    
+  Inductive step : state -> option observation -> state -> Prop :=
+  | StepEquivState : forall st1 st2,
+    st1 === st2 ->
+    step st1 None st2
+  | PktProcess : forall swId pts tbl pt pk inp outp ctrlm switchm outp'
+                        pksToCtrl,
+    process_packet tbl pt pk = (outp', pksToCtrl) ->
+    SwitchStep[
+      Switch swId pts tbl ({|(pt,pk)|} <+> inp) outp ctrlm switchm;
+      Some (swId,pt,pk);
+      Switch swId pts tbl inp (FromList outp' <+> outp) 
+        ctrlm (FromList (map (PacketIn pt) pksToCtrl) <+> switchm)
+    ]
+  | ModifyFlowTable : forall swId pts tbl inp outp fm ctrlm switchm,
+    SwitchStep[
+      Switch swId pts tbl inp outp ({|FlowMod fm|} <+> ctrlm) switchm;
+      None;
+      Switch swId pts (modify_flow_table fm tbl) inp outp ctrlm switchm
+    ]
+  | SendPacketOut : forall pt pts swId tbl inp outp pk ctrlm switchm,
+    In pt pts ->
+    SwitchStep[
+      Switch swId pts tbl inp outp  ({|PacketOut pt pk|} <+> ctrlm) switchm;
+      None;
+      Switch swId pts tbl inp ({| (pt,pk) |} <+> outp) ctrlm switchm
+    ]
+  | SendDataLink : forall swId pts tbl inp pt pk outp ctrlm switchm pks dst,
+    TopoStep[
+      Switch swId pts tbl inp ({|(pt,pk)|} <+> outp) ctrlm switchm;
+      DataLink (swId,pt) pks dst;
+      None;
+      Switch swId pts tbl inp outp ctrlm switchm;
+      DataLink (swId,pt) (pk :: pks) dst
+    ]
+  | RecvDataLink : forall swId pts tbl inp outp ctrlm switchm src pks pk pt,
+    TopoStep[
+      Switch swId pts tbl inp outp ctrlm switchm;
+      DataLink src  (pks ++ [pk]) (swId,pt);
+      None;
+      Switch swId pts tbl ({|(pt,pk)|} <+> inp) outp ctrlm switchm;
+      DataLink src pks (swId,pt)
+    ]
+  | Step_controller : forall sws links ofLinks ctrl ctrl',
+    controller_step ctrl ctrl' ->
+    step (State sws links ofLinks ctrl)
+         None
+         (State sws links ofLinks ctrl')
+  | ControllerRecv : forall ctrl msg ctrl' swId fromSwitch fromCtrl,
+    controller_recv ctrl swId msg ctrl' ->
+    ControllerOpenFlow[
+      ctrl;
+      OpenFlowLink swId (fromSwitch ++ [msg]) fromCtrl;
+      None;
+      ctrl';
+      OpenFlowLink swId fromSwitch fromCtrl
+    ]
+  | ControllerSend : forall ctrl msg ctrl' swId fromSwitch fromCtrl,
+    controller_send ctrl ctrl' swId msg ->
+    ControllerOpenFlow[
+      ctrl ;
+      (OpenFlowLink swId fromSwitch fromCtrl);
+      None;
+      ctrl';
+      (OpenFlowLink swId fromSwitch (msg :: fromCtrl)) ]
+  | SendToController : forall swId pts tbl inp outp ctrlm msg switchm fromSwitch
+      fromCtrl,
+    SwitchOpenFlow[
+      Switch swId pts tbl inp outp ctrlm ({| msg |} <+> switchm);
+      OpenFlowLink swId fromSwitch fromCtrl;
+      None;
+      Switch swId pts tbl inp outp ctrlm switchm;
+      OpenFlowLink swId (msg :: fromSwitch) fromCtrl
+    ]
+  | RecvBarrier : forall swId pts tbl inp outp switchm fromSwitch fromCtrl
+      xid,
+    SwitchOpenFlow[
+      Switch swId pts tbl inp outp Empty switchm;
+      OpenFlowLink swId fromSwitch (fromCtrl ++ [BarrierRequest xid]);
+      None;
+      Switch swId pts tbl inp outp Empty
+             ({| BarrierReply xid |} <+> switchm);
+      OpenFlowLink swId fromSwitch fromCtrl
+    ]
+  | RecvFromController : forall swId pts tbl inp outp ctrlm switchm
+      fromSwitch fromCtrl msg,
+    NotBarrierRequest msg ->
+    SwitchOpenFlow[
+      Switch swId pts tbl inp outp ctrlm switchm;
+      OpenFlowLink swId fromSwitch (fromCtrl ++ [msg]);
+      None;
+      Switch swId pts tbl inp outp ({| msg |} <+> ctrlm) switchm;
+      OpenFlowLink swId fromSwitch fromCtrl
+    ]
+      where
+  "ControllerOpenFlow[ c ; l ; obs ; c0 ; l0 ]" := 
+    (forall sws links ofLinks ofLinks',
+      step (State sws links (ofLinks ++ l :: ofLinks') c) 
+           obs 
+           (State sws links (ofLinks ++ l0 :: ofLinks') c0))
+    and
+  "TopoStep[ sw ; link ; obs ; sw0 ; link0 ]" :=
+    (forall sws links links0 ofLinks ctrl,
+      step 
+      (State (({|sw|}) <+> sws) (links ++ link :: links0) ofLinks ctrl)
+      obs
+      (State (({|sw0|}) <+> sws) (links ++ link0 :: links0) ofLinks ctrl))
+    and
+  "SwitchStep[ sw ; obs ; sw0 ]" :=
+    (forall sws links ofLinks ctrl,
+      step 
+        (State (({|sw|}) <+> sws) links ofLinks ctrl)
+        obs
+        (State (({|sw0|}) <+> sws) links ofLinks ctrl))
+    and
+  "SwitchOpenFlow[ sw ; of ; obs ; sw0 ; of0 ]" :=
+    (forall sws links ofLinks ofLinks0 ctrl,
+      step
+        (State (({|sw|}) <+> sws) links (ofLinks ++ of :: ofLinks0) ctrl)
+        obs
+        (State (({|sw0|}) <+> sws) links (ofLinks ++ of0 :: ofLinks0) ctrl)).
+
+  Definition abst_state := bag (switchId * portId * packet).
+
+  Definition transfer (sw : switchId) (ptpk : portId * packet) :=
+    match ptpk with
+      | (pt,pk) =>
+        match topo (sw,pt) with
+          | Some (sw',pt') => {| (sw',pt',pk) |}
+          | None => {| |}
+        end
+    end.
+
+  Definition select_packet_out (sw : switchId) (msg : fromController) :=
+    match msg with
+      | PacketOut pt pk => transfer sw (pt,pk)
+      | _ => {| |}
+    end.
+
+  Definition select_packet_in (sw : switchId) (msg : fromSwitch) :=
+    match msg with
+      | PacketIn pt pk => Bag.unions (map (transfer sw) (abst_func sw pt pk))
+      | _ => {| |}
+    end.
+
+  Definition FlowTableSafe (sw : switchId) (tbl : flowTable) : Prop :=
+    forall pt pk forwardedPkts packetIns,
+      process_packet tbl pt pk = (forwardedPkts, packetIns) ->
+      Bag.unions (map (transfer sw) forwardedPkts) <+>
+      Bag.unions (map (select_packet_in sw) (map (PacketIn pt) packetIns)) ===
+      Bag.unions (map (transfer sw) (abst_func sw pt pk)).
+
+  Section FlowModSafety.
+
+    Inductive Endpoint : Type :=
+    | Endpoint_NoBarrier : flowTable -> Endpoint
+    | Endpoint_Barrier : flowTable -> Endpoint.
+
+    Definition table_at_endpoint (ep : Endpoint) :=
+      match ep with
+        | Endpoint_NoBarrier tbl => tbl
+        | Endpoint_Barrier tbl => tbl
+      end.
+
+    Inductive SafeWire : switchId -> 
+                    Endpoint -> 
+                    list fromController ->
+                    Endpoint -> Prop :=
+    | SafeWire_nil : forall swId ep,
+      FlowTableSafe swId (table_at_endpoint ep) ->
+      SafeWire swId ep nil ep
+    | SafeWire_PktOut : forall swId pt pk ctrlEp ctrlm swEp,
+      SafeWire swId ctrlEp ctrlm swEp ->
+      SafeWire swId ctrlEp (PacketOut pt pk :: ctrlm) swEp
+    | SafeWire_BarrierRequest : forall swId n ctrlEp ctrlm swEp,
+      SafeWire swId ctrlEp ctrlm swEp ->
+      SafeWire swId (Endpoint_Barrier (table_at_endpoint ctrlEp))
+                    (BarrierRequest n :: ctrlm)
+                    swEp
+    | SafeWire_FlowMod : forall swId f tbl ctrlm swEp,
+      FlowTableSafe swId (modify_flow_table f tbl) ->
+      SafeWire swId (Endpoint_Barrier tbl) ctrlm swEp ->
+      SafeWire swId (Endpoint_NoBarrier (modify_flow_table f tbl))
+          (FlowMod f :: ctrlm) swEp.
+
+    Inductive NotFlowMod : fromController -> Prop :=
+    | NotFlowMod_BarrierRequest : forall n, NotFlowMod (BarrierRequest n)
+    | NotFlowMod_PacketOut : forall pt pk, NotFlowMod (PacketOut pt pk).
+
+    Inductive SwitchEP : switch -> Endpoint -> Prop :=
+    | NoFlowModsInBuffer : forall swId pts tbl inp outp ctrlm switchm swEp,
+      (forall msg, Mem msg ctrlm -> NotFlowMod msg) ->
+      table_at_endpoint swEp = tbl ->
+      SwitchEP
+        (Switch swId pts tbl inp outp ctrlm switchm)
+        swEp
+    | OneFlowModInBuffer : forall swId pts tbl inp outp ctrlm ctrlm0 switchm f,
+      (forall msg, Mem msg ctrlm0 -> NotFlowMod msg) ->
+      ctrlm === ({|FlowMod f|} <+> ctrlm0) ->
+      FlowTableSafe swId (modify_flow_table f tbl) ->
+      SwitchEP (Switch swId pts tbl inp outp ctrlm switchm)
+               (Endpoint_NoBarrier (modify_flow_table f tbl)).
+
+    (** "FMS" is short for "flow mod safety". *)
+    Inductive FMS : switch -> openFlowLink -> Prop := 
+    | MkFMS : forall swId pts tbl inp outp ctrlm switchm ctrlmList switchmList
+                     switchEp,
+      SwitchEP (Switch swId pts tbl inp outp ctrlm switchm) switchEp ->
+      (exists ctrlEp, SafeWire swId ctrlEp ctrlmList switchEp) ->
+      FMS 
+        (Switch swId pts tbl inp outp ctrlm switchm)
+        (OpenFlowLink swId switchmList ctrlmList).
+
+    Definition AllFMS (sws : bag switch) (ofLinks : list openFlowLink) :=
+      forall sw,
+        Mem sw sws ->
+        exists lnk, 
+          In lnk ofLinks /\
+          of_to lnk = swId sw /\
+          FMS sw lnk.
+
+    Parameter SwitchEP_equiv : forall swId pts tbl inp0 inp1 outp0 outp1
+      ctrlm0 ctrlm1 switchm0 switchm1 ep,
+      ctrlm0 === ctrlm1 ->
+      SwitchEP (Switch swId pts tbl inp0 outp0 ctrlm0 switchm0) ep ->
+      SwitchEP (Switch swId pts tbl inp1 outp1 ctrlm1 switchm1) ep.
+
+    Parameter FMS_untouched : forall swId0 pts0 tbl0 inp0 outp0 ctrlm0 switchm0
+      switchmLst0 ctrlmLst0 inp1 outp1 switchm1 switchmLst1,
+      FMS (Switch swId0 pts0 tbl0 inp0 outp0 ctrlm0 switchm0)
+          (OpenFlowLink swId0 switchmLst0 ctrlmLst0) ->
+      FMS (Switch swId0 pts0 tbl0 inp1 outp1 ctrlm0 switchm1)
+          (OpenFlowLink swId0 switchmLst1 ctrlmLst0).
+
+    Parameter FMS_equiv : forall sw1 sw2 lnk,
+      sw1 === sw2 ->
+      FMS sw1 lnk ->
+      FMS sw2 lnk.
+
+    Parameter SafeWire_dequeue_PacketOut : forall sw ctrlEp ctrlLst pt pk 
+      switchEp,
+      SafeWire sw ctrlEp (ctrlLst ++ [PacketOut pt pk]) switchEp ->
+      SafeWire sw ctrlEp (ctrlLst) switchEp.
+
+    Parameter SafeWire_dequeue_BarrierRequest : forall sw ctrlEp ctrlLst xid 
+      switchEp1,
+      SafeWire sw ctrlEp (ctrlLst ++ [BarrierRequest xid]) switchEp1 ->
+      exists switchEp2, SafeWire sw ctrlEp (ctrlLst) switchEp2 /\
+        table_at_endpoint switchEp2 = table_at_endpoint switchEp1.
+
+    Parameter SafeWire_dequeue_safe : forall sw ctrlEp ctrlLst f switchEp,
+       SafeWire sw ctrlEp (ctrlLst ++ [FlowMod f]) switchEp ->
+       FlowTableSafe sw (modify_flow_table f (table_at_endpoint switchEp)).
+
+    Parameter SafeWire_dequeue_FlowMod : forall sw ctrlEp ctrlLst f switchEp,
+       SafeWire sw ctrlEp (ctrlLst ++ [FlowMod f]) switchEp ->
+       SafeWire sw ctrlEp ctrlLst 
+                (Endpoint_NoBarrier 
+                   (modify_flow_table f
+                     (table_at_endpoint switchEp))).
+
+    Parameter SafeWire_fm_nb_false : forall sw ctrlEp ctrlLst f tbl,
+      SafeWire sw ctrlEp (ctrlLst ++ [FlowMod f]) (Endpoint_NoBarrier tbl) ->
+      False.
+
+    Parameter FMS_pop : forall sw pts tbl inp outp ctrlm switchm switchLst 
+                               ctrlLst msg,
+      FMS  (Switch sw pts tbl inp outp ctrlm switchm) 
+           (OpenFlowLink sw switchLst (ctrlLst ++ [msg])) ->
+      FMS  (Switch sw pts tbl inp outp ({|msg|} <+> ctrlm) switchm) 
+           (OpenFlowLink sw switchLst ctrlLst).
+
+    Parameter FMS_dequeue_pktOut : forall sw pts tbl inp outp ctrlm switchm 
+                                      switchLst ctrlLst pt pk,
+      FMS  (Switch sw pts tbl inp outp ({|PacketOut pt pk|} <+> ctrlm) switchm)
+           (OpenFlowLink sw switchLst ctrlLst) ->
+      FMS  (Switch sw pts tbl inp ({|(pt,pk)|} <+> outp) ctrlm switchm) 
+           (OpenFlowLink sw switchLst ctrlLst).
+
+  End FlowModSafety.
+
+End MACHINE.
+
+Module Type ATOMS_AND_CONTROLLER.
+
+  Declare Module Machine : MACHINE.
+  Import Machine.
+  Import Atoms.
+
+  Parameter relate_controller : controller -> bag (switchId * portId * packet).
+
+  Parameter ControllerRemembersPackets :
+    forall (ctrl ctrl' : controller),
+      controller_step ctrl ctrl' ->
+      relate_controller ctrl = relate_controller ctrl'.
+
+  Parameter P : bag switch -> list openFlowLink -> controller -> Prop.
+  
+  Parameter step_preserves_P : forall sws0 sws1 links0 links1 ofLinks0 ofLinks1 
+    ctrl0 ctrl1 obs,
+    step (State sws0 links0 ofLinks0 ctrl0)
+         obs
+         (State sws1 links1 ofLinks1 ctrl1) ->
+    P sws0 ofLinks0 ctrl0 ->
+    P sws1 ofLinks1 ctrl1.
+
+  Parameter ControllerSendForgetsPackets : forall ctrl ctrl' sw msg,
+    controller_send ctrl ctrl' sw msg ->
+    relate_controller ctrl === select_packet_out sw msg <+>
+    relate_controller ctrl'.
+
+  Parameter ControllerRecvRemembersPackets : forall ctrl ctrl' sw msg,
+    controller_recv ctrl sw msg ctrl' ->
+    relate_controller ctrl' === select_packet_in sw msg <+> 
+    (relate_controller ctrl).
+
+  Parameter ControllerLiveness : forall sw pt pk ctrl0 sws0 links0 ofLinks0,
+    Mem (sw,pt,pk) (relate_controller ctrl0) ->
+    exists  ofLinks10 ofLinks11 ctrl1 swTo ptTo switchmLst ctrlmLst,
+      (multistep 
+         step (State sws0 links0 ofLinks0 ctrl0) nil
+         (State sws0 links0
+                (ofLinks10 ++ 
+                 (OpenFlowLink swTo switchmLst 
+                  (PacketOut ptTo pk :: ctrlmLst)) ::
+                 ofLinks11) 
+                ctrl1)) /\
+      select_packet_out swTo (PacketOut ptTo pk) = ({|(sw,pt,pk)|}).
+
+  Parameter ControllerFMS : forall swId ctrl0 ctrl1 msg ctrlm
+    switchm sws links ofLinks0 ofLinks1 switchEp
+    pts tbl inp outp swCtrlm swSwitchm,
+    P sws
+      (ofLinks0 ++ (OpenFlowLink swId switchm ctrlm) :: ofLinks1)
+      ctrl0 ->
+    controller_send ctrl0 ctrl1 swId msg ->
+    step
+      (State
+        sws
+        links
+        (ofLinks0 ++ (OpenFlowLink swId switchm ctrlm) :: ofLinks1)
+        ctrl0)
+      None
+      (State
+         sws
+         links
+         (ofLinks0 ++ (OpenFlowLink swId switchm (msg :: ctrlm)) :: ofLinks1)
+         ctrl1) ->
+     Mem (Switch swId pts tbl inp outp swCtrlm swSwitchm) sws ->
+     SwitchEP (Switch swId pts tbl inp outp swCtrlm swSwitchm) switchEp ->
+      exists ctrlEp1,
+        SafeWire swId ctrlEp1 (msg :: ctrlm) switchEp.
+
+End ATOMS_AND_CONTROLLER.
+
+Module Type RELATION.
+
+  Declare Module AtomsAndController : ATOMS_AND_CONTROLLER.
+  Export AtomsAndController.
+  Export Machine.
+  Export Atoms.
+
+  Definition affixSwitch (sw : switchId) (ptpk : portId * packet) :=
+    match ptpk with
+      | (pt,pk) => (sw,pt,pk)
+    end.
+
+  Definition FlowTablesSafe (sws : bag switch) : Prop :=
+    forall swId pts tbl inp outp ctrlm switchm,
+      Mem (Switch swId pts tbl inp outp ctrlm switchm) sws ->
+      FlowTableSafe swId tbl.
+
+  Definition ConsistentDataLinks (links : list dataLink) : Prop :=
+    forall (lnk : dataLink),
+      In lnk links ->
+      topo (src lnk) = Some (dst lnk).
+
+  Definition LinkHasSrc (sws : bag switch) (link : dataLink) : Prop :=
+    exists switch,
+      Mem switch sws /\
+      fst (src link) = swId switch /\
+      In (snd (src link)) (pts switch).
+
+  Definition LinkHasDst (sws : bag switch) (link : dataLink) : Prop :=
+    exists switch,
+      Mem switch sws /\
+      fst (dst link) = swId switch /\
+      In (snd (dst link)) (pts switch).
+
+  Definition LinksHaveSrc (sws : bag switch) (links : list dataLink) :=
+    forall link, In link links -> LinkHasSrc sws link.
+
+  Definition LinksHaveDst (sws : bag switch) (links : list dataLink) :=
+    forall link, In link links -> LinkHasDst sws link.
+
+  Definition UniqSwIds (sws : bag switch) := AllDiff swId (Bag.to_list sws).
+
+  Definition ofLinkHasSw (sws : bag switch) (ofLink : openFlowLink) :=
+    exists sw,
+      Mem sw sws /\
+      of_to ofLink = swId sw.
+
+  Definition OFLinksHaveSw (sws : bag switch) (ofLinks : list openFlowLink) :=
+    forall ofLink, In ofLink ofLinks -> ofLinkHasSw sws ofLink.
+
+  Record concreteState := ConcreteState {
+    devices : state;
+    concreteState_flowTableSafety : FlowTablesSafe (switches devices);
+    concreteState_consistentDataLinks : ConsistentDataLinks (links devices);
+    linksHaveSrc : LinksHaveSrc (switches devices) (links devices);
+    linksHaveDst : LinksHaveDst (switches devices) (links devices);
+    uniqSwIds : UniqSwIds (switches devices);
+    allFMS : AllFMS (switches devices) (ofLinks devices);
+    ctrlP : P (switches devices) (ofLinks devices) (ctrl devices);
+    uniqOfLinkIds : AllDiff of_to (ofLinks devices);
+    ofLinksHaveSw : OFLinksHaveSw (switches devices) (ofLinks devices)
+  }.
+
+  Implicit Arguments ConcreteState [].
+
+  Definition concreteStep (st : concreteState) (obs : option observation)
+    (st0 : concreteState) :=
+    step (devices st) obs (devices st0).
+
+  Inductive abstractStep : abst_state -> option observation -> abst_state -> 
+    Prop := 
+  | AbstractStepEquiv : forall st st',
+      st === st' ->
+      abstractStep st None st'
+  | AbstractStep : forall sw pt pk lps,
+    abstractStep
+      ({| (sw,pt,pk) |} <+> lps)
+      (Some (sw,pt,pk))
+      (Bag.unions (map (transfer sw) (abst_func sw pt pk)) <+> lps).
+
+  Definition relate_switch (sw : switch) : abst_state :=
+    match sw with
+      | Switch swId _ tbl inp outp ctrlm switchm =>
+        FromList (map (affixSwitch swId) (Bag.to_list inp)) <+>
+        Bag.unions (map (transfer swId) (Bag.to_list outp)) <+>
+        Bag.unions (map (select_packet_out swId) (Bag.to_list ctrlm)) <+>
+        Bag.unions (map (select_packet_in swId) (Bag.to_list switchm))
+    end.
+
+  Definition relate_dataLink (link : dataLink) : abst_state :=
+    match link with
+      | DataLink _ pks (sw,pt) =>
+        FromList (map (fun pk => (sw,pt,pk)) pks)
+    end.
+
+  Definition relate_openFlowLink (link : openFlowLink) : abst_state :=
+    match link with
+      | OpenFlowLink sw switchm ctrlm =>
+        Bag.unions (map (select_packet_out sw) ctrlm) <+>
+        Bag.unions (map (select_packet_in sw) switchm)
+    end.
+
+
+  Definition relate (st : state) : abst_state :=
+    Bag.unions (map relate_switch (Bag.to_list (switches st))) <+>
+    Bag.unions (map relate_dataLink (links st)) <+>
+    Bag.unions (map relate_openFlowLink (ofLinks st)) <+>
+    relate_controller (ctrl st).
+
+  Definition bisim_relation : relation concreteState abst_state :=
+    fun (st : concreteState) (ast : abst_state) => 
+      ast === (relate (devices st)).
+
+  Parameter simpl_multistep : forall (st1 st2 : state) obs
+    (tblsOk1 : FlowTablesSafe (switches st1))
+    (linksTopoOk1 : ConsistentDataLinks (links st1))
+    (haveSrc1 : LinksHaveSrc (switches st1) (links st1))
+    (haveDst1 : LinksHaveDst (switches st1) (links st1))
+    (uniqSwIds1 : UniqSwIds (switches st1))
+    (allFMS1 : AllFMS (switches st1) (ofLinks st1))
+    (P1 : P (switches st1) (ofLinks st1) (ctrl st1))
+    (uniqOfLinkIds1 : AllDiff of_to (ofLinks st1))
+    (ofLinksHaveSw1 : OFLinksHaveSw (switches st1) (ofLinks st1)),
+    multistep step st1 obs st2 ->
+    exists tblsOk2 linksTopoOk2 haveSrc2 haveDst2 uniqSwIds2 allFMS2 P2
+           uniqOfLinkIds2 ofLinksHaveSw2,
+      multistep concreteStep
+                (ConcreteState st1 tblsOk1 linksTopoOk1 haveSrc1 haveDst1 
+                               uniqSwIds1 allFMS1 P1 uniqOfLinkIds1
+                               ofLinksHaveSw1)
+                obs
+                (ConcreteState st2 tblsOk2 linksTopoOk2 haveSrc2 haveDst2 
+                               uniqSwIds2 allFMS2 P2 uniqOfLinkIds2
+                               ofLinksHaveSw2).
+
+
+  Parameter simpl_weak_sim : forall devs1 devs2 sw pt pk lps
+    (tblsOk1 : FlowTablesSafe (switches devs1))
+    (linksTopoOk1 : ConsistentDataLinks (links devs1))
+    (haveSrc1 : LinksHaveSrc (switches devs1) (links devs1))
+    (haveDst1 : LinksHaveDst (switches devs1) (links devs1))
+    (uniqSwIds1 : UniqSwIds (switches devs1))
+    (allFMS1 : AllFMS (switches devs1) (ofLinks devs1))
+    (P1 : P (switches devs1) (ofLinks devs1) (ctrl devs1))
+    (uniqOfLinkIds1 : AllDiff of_to (ofLinks devs1))
+    (ofLinksHaveSw1 : OFLinksHaveSw (switches devs1) (ofLinks devs1)),
+    multistep step devs1 [(sw,pt,pk)] devs2 ->
+    relate devs1 === ({| (sw,pt,pk) |} <+> lps) ->
+    abstractStep
+      ({| (sw,pt,pk) |} <+> lps)
+      (Some (sw,pt,pk))
+      (Bag.unions (map (transfer sw) (abst_func sw pt pk)) <+> lps) ->
+   exists t : concreteState,
+     inverse_relation 
+       bisim_relation
+       (Bag.unions (map (transfer sw) (abst_func sw pt pk)) <+> lps)
+       t /\
+     multistep concreteStep
+               (ConcreteState devs1 tblsOk1 linksTopoOk1 haveSrc1 haveDst1
+                              uniqSwIds1 allFMS1 P1 uniqOfLinkIds1
+                              ofLinksHaveSw1)
+               [(sw,pt,pk)]
+               t.
+
+  Parameter FlowTablesSafe_untouched : forall {sws swId pts tbl inp inp'
+    outp outp' ctrlm ctrlm' switchm switchm' },
+    FlowTablesSafe
+      ({|Switch swId pts tbl inp outp ctrlm switchm|} <+> sws) ->
+    FlowTablesSafe 
+      ({|Switch swId pts tbl inp' outp' ctrlm' switchm'|} <+> sws).
+
+  Parameter LinksHaveSrc_untouched : forall 
+    {swId tbl pts sws links
+    inp outp ctrlm switchm tbl' inp' outp' ctrlm' switchm' },
+    LinksHaveSrc 
+      ({| Switch swId pts tbl inp outp ctrlm switchm |} <+> sws)  links ->
+    LinksHaveSrc 
+      ({| Switch swId pts tbl' inp' outp' ctrlm' switchm' |} <+> sws)
+      links.
+
+  Parameter LinkHasSrc_equiv : forall {sws sws' link},
+    sws === sws' ->
+    LinkHasSrc sws link ->
+    LinkHasSrc sws' link.
+
+  Parameter LinksHaveDst_untouched : forall 
+    {swId tbl pts sws links
+    inp outp ctrlm switchm tbl' inp' outp' ctrlm' switchm' },
+    LinksHaveDst
+      ({| Switch swId pts tbl inp outp ctrlm switchm |} <+>  sws)  links ->
+    LinksHaveDst 
+      ({| Switch swId pts tbl' inp' outp' ctrlm' switchm' |} <+> sws)
+      links.
+
+  Parameter LinkHasDst_equiv : forall {sws sws' link},
+    sws === sws' ->
+    LinkHasDst sws link ->
+    LinkHasDst sws' link.
+
+End RELATION.
+
+Module Type WEAK_SIM_1.
+
+  Declare Module Relation : RELATION.
+  Import Relation.
+  
+  Parameter weak_sim_1 : weak_simulation concreteStep abstractStep bisim_relation.
+
+End WEAK_SIM_1.
+
+Module Type WEAK_SIM_2.
+
+  Declare Module Relation : RELATION.
+  Import Relation.
+  
+  Parameter weak_sim_2 :
+    weak_simulation abstractStep concreteStep (inverse_relation bisim_relation).
+
+End WEAK_SIM_2.
