coq/FwOF/FwOFWellFormedness.v
@@ -7,21 +7,126 @@ Require Import Coq.Classes.Morphisms.
 Require Import Coq.Setoids.Setoid.
 Require Import Common.Types.
 Require Import Common.Bisimulation.
-Require Import Bag.Bag.
-Require Import FwOF.FwOF.
-Require FwOF.FwOFRelation.
 Require Import Common.AllDiff.
+Require Import Bag.Bag.
+Require Import FwOF.FwOFSignatures.
 
 Local Open Scope list_scope.
 Local Open Scope equiv_scope.
 Local Open Scope bag_scope.
 
-Module Make (AtomsAndController : ATOMS_AND_CONTROLLER).
+Module Make (AtomsAndController_ : ATOMS_AND_CONTROLLER) <: RELATION.
 
+  Module AtomsAndController := AtomsAndController_.
   Import AtomsAndController.
+  Import Machine.
   Import Atoms.
-  Import FwOF.
-  Module Import Relation := FwOF.FwOFRelation.Make (AtomsAndController).
+
+  Definition affixSwitch (sw : switchId) (ptpk : portId * packet) :=
+    match ptpk with
+      | (pt,pk) => (sw,pt,pk)
+    end.
+
+  Definition FlowTablesSafe (sws : bag switch) : Prop :=
+    forall swId pts tbl inp outp ctrlm switchm,
+      Mem (Switch swId pts tbl inp outp ctrlm switchm) sws ->
+      FlowTableSafe swId tbl.
+
+  Definition ConsistentDataLinks (links : list dataLink) : Prop :=
+    forall (lnk : dataLink),
+      In lnk links ->
+      topo (src lnk) = Some (dst lnk).
+
+  Definition LinkHasSrc (sws : bag switch) (link : dataLink) : Prop :=
+    exists switch,
+      Mem switch sws /\
+      fst (src link) = swId switch /\
+      In (snd (src link)) (pts switch).
+
+  Definition LinkHasDst (sws : bag switch) (link : dataLink) : Prop :=
+    exists switch,
+      Mem switch sws /\
+      fst (dst link) = swId switch /\
+      In (snd (dst link)) (pts switch).
+
+  Definition LinksHaveSrc (sws : bag switch) (links : list dataLink) :=
+    forall link, In link links -> LinkHasSrc sws link.
+
+  Definition LinksHaveDst (sws : bag switch) (links : list dataLink) :=
+    forall link, In link links -> LinkHasDst sws link.
+
+  Definition UniqSwIds (sws : bag switch) := AllDiff swId (Bag.to_list sws).
+
+  Definition ofLinkHasSw (sws : bag switch) (ofLink : openFlowLink) :=
+    exists sw,
+      Mem sw sws /\
+      of_to ofLink = swId sw.
+
+  Definition OFLinksHaveSw (sws : bag switch) (ofLinks : list openFlowLink) :=
+    forall ofLink, In ofLink ofLinks -> ofLinkHasSw sws ofLink.
+
+  Record concreteState := ConcreteState {
+    devices : state;
+    concreteState_flowTableSafety : FlowTablesSafe (switches devices);
+    concreteState_consistentDataLinks : ConsistentDataLinks (links devices);
+    linksHaveSrc : LinksHaveSrc (switches devices) (links devices);
+    linksHaveDst : LinksHaveDst (switches devices) (links devices);
+    uniqSwIds : UniqSwIds (switches devices);
+    allFMS : AllFMS (switches devices) (ofLinks devices);
+    ctrlP : P (switches devices) (ofLinks devices) (ctrl devices);
+    uniqOfLinkIds : AllDiff of_to (ofLinks devices);
+    ofLinksHaveSw : OFLinksHaveSw (switches devices) (ofLinks devices)
+  }.
+
+  Implicit Arguments ConcreteState [].
+
+  Definition concreteStep (st : concreteState) (obs : option observation)
+    (st0 : concreteState) :=
+    step (devices st) obs (devices st0).
+
+  Inductive abstractStep : abst_state -> option observation -> abst_state -> 
+    Prop := 
+  | AbstractStepEquiv : forall st st',
+      st === st' ->
+      abstractStep st None st'
+  | AbstractStep : forall sw pt pk lps,
+    abstractStep
+      ({| (sw,pt,pk) |} <+> lps)
+      (Some (sw,pt,pk))
+      (Bag.unions (map (transfer sw) (abst_func sw pt pk)) <+> lps).
+
+  Definition relate_switch (sw : switch) : abst_state :=
+    match sw with
+      | Switch swId _ tbl inp outp ctrlm switchm =>
+        FromList (map (affixSwitch swId) (Bag.to_list inp)) <+>
+        Bag.unions (map (transfer swId) (Bag.to_list outp)) <+>
+        Bag.unions (map (select_packet_out swId) (Bag.to_list ctrlm)) <+>
+        Bag.unions (map (select_packet_in swId) (Bag.to_list switchm))
+    end.
+
+  Definition relate_dataLink (link : dataLink) : abst_state :=
+    match link with
+      | DataLink _ pks (sw,pt) =>
+        FromList (map (fun pk => (sw,pt,pk)) pks)
+    end.
+
+  Definition relate_openFlowLink (link : openFlowLink) : abst_state :=
+    match link with
+      | OpenFlowLink sw switchm ctrlm =>
+        Bag.unions (map (select_packet_out sw) ctrlm) <+>
+        Bag.unions (map (select_packet_in sw) switchm)
+    end.
+
+
+  Definition relate (st : state) : abst_state :=
+    Bag.unions (map relate_switch (Bag.to_list (switches st))) <+>
+    Bag.unions (map relate_dataLink (links st)) <+>
+    Bag.unions (map relate_openFlowLink (ofLinks st)) <+>
+    relate_controller (ctrl st).
+
+  Definition bisim_relation : relation concreteState abst_state :=
+    fun (st : concreteState) (ast : abst_state) => 
+      ast === (relate (devices st)).
 
   Lemma LinksHaveSrc_untouched : forall 
     {swId tbl pts sws links
